02Stack/EvaluateStack.thy
@@ -1,0 +1,109 @@
+theory EvaluateStack
+imports TypecheckStack
+begin
+
+inductive evaluate :: "stack_state \<Rightarrow> stack_state \<Rightarrow> bool" (infix "\<leadsto>\<^sub>s" 60) where
+  ev_abs [simp]: "StackState Eval (Abs t e) s h \<leadsto>\<^sub>s StackState Return (Abs t e) s h"
+| ev_app [simp]: "StackState Eval (App e\<^sub>1 e\<^sub>2) s h \<leadsto>\<^sub>s StackState Eval e\<^sub>1 (SApp e\<^sub>2 # s) h" 
+| ev_let [simp]: "StackState Eval (Let e\<^sub>1 e\<^sub>2) s h \<leadsto>\<^sub>s StackState Eval e\<^sub>2' (SBind # s) (e\<^sub>1 # h)"
+| ev_rec [simp]: "list_all is_var vs \<Longrightarrow> \<not> is_var e \<Longrightarrow> 
+    StackState Eval (Rec (vs @ [e] @ nvs)) s h \<leadsto>\<^sub>s 
+      StackState Eval (Rec (map (incr\<^sub>e\<^sub>e 0) vs @ [Var 0] @ map (incr\<^sub>e\<^sub>e 0) nvs)) (SBind # s) (e # h)" 
+| ev_rec2 [simp]: "list_all is_var vs \<Longrightarrow> \<not> is_var e \<Longrightarrow> 
+    StackState Eval (Rec vs) s h \<leadsto>\<^sub>s StackState Return (Rec vs) s h" 
+| ev_proj [simp]: "StackState Eval (Proj e l) s h \<leadsto>\<^sub>s StackState Eval e (SProj l # s) h"
+| ev_inj [simp]: "StackState Eval (Inj l ts e) s h \<leadsto>\<^sub>s 
+    StackState Return (if is_var e then Inj l ts e else Inj l ts (Var 0)) s h"
+| ev_case [simp]: "StackState Eval (Case e t cs) s h \<leadsto>\<^sub>s StackState Eval e (SCase t cs # s) h"
+| ev_fold [simp]: "StackState Eval (Fold t e) s h \<leadsto>\<^sub>s 
+    StackState Return (if is_var e then Fold t e else Let e (Fold t (Var 0))) s h" 
+| ev_unfold [simp]: "StackState Eval (Unfold t e) s h \<leadsto>\<^sub>s StackState Eval e (SUnfold t # s) h"  
+| ev_tyabs [simp]: "StackState Eval (TyAbs k e) s h \<leadsto>\<^sub>s StackState Return (TyAbs k e) s h" 
+| ev_tyapp [simp]: "StackState Eval (TyApp e t) s h \<leadsto>\<^sub>s StackState Eval e (STyApp t # s) h" 
+| ev_tylet [simp]: "StackState Eval (TyLet t e) s h \<leadsto>\<^sub>s StackState Eval (subst\<^sub>t\<^sub>e 0 t e) s h" 
+| ret_app [simp]: 
+    "StackState Return (Abs t e\<^sub>1) (SApp e\<^sub>2 # s) h \<leadsto>\<^sub>s StackState Eval e\<^sub>1 (SBind # s) (e\<^sub>2 # h)"
+| ret_proj [simp]: "lookup l fs = Some e \<Longrightarrow> 
+    StackState Return (Rec fs) (SProj l # s) h \<leadsto>\<^sub>s StackState Eval e s h" 
+| ret_case [simp]: "lookup l cs = Some e' \<Longrightarrow> 
+    StackState Return (Inj l ts e) (SCase t cs # s) h \<leadsto>\<^sub>s StackState Eval e' (SBind # s) (e # h)"
+| ret_unfold [simp]: "StackState Return (Fold t e) (SUnfold t # s) h \<leadsto>\<^sub>s StackState Eval e s h" 
+| ret_tyapp [simp]: 
+    "StackState Return (TyAbs k e) (STyApp t # s) h \<leadsto>\<^sub>s StackState Eval (subst\<^sub>t\<^sub>e 0 t e) s h" 
+| ret_app_let [simp]: "StackState Return (Let e\<^sub>1\<^sub>1 e\<^sub>1\<^sub>2) (SApp e\<^sub>2 # s) h \<leadsto>\<^sub>s 
+    StackState Eval e\<^sub>1\<^sub>2 (SApp (incr\<^sub>e\<^sub>e 0 e\<^sub>2) # SBind # s) (e\<^sub>1\<^sub>1 # h)"
+| ret_proj_let [simp]: "StackState Return (Let e\<^sub>1 e\<^sub>2) (SProj l # s) h \<leadsto>\<^sub>s 
+    StackState Eval e\<^sub>2 (SProj l # SBind # s) (e\<^sub>1 # h)" 
+| ret_case_let [simp]: "StackState Return (Let e\<^sub>1 e\<^sub>2) (SCase t cs # s) h \<leadsto>\<^sub>s 
+    StackState Eval e\<^sub>2 (SCase t (map (incr\<^sub>e\<^sub>e (Suc 0)) cs) # SBind # s) (e\<^sub>1 # h)" 
+| ret_unfold_let [simp]: "StackState Return (Let e\<^sub>1 e\<^sub>2) (SUnfold t # s) h \<leadsto>\<^sub>s 
+    StackState Eval e\<^sub>2 (SUnfold t # SBind # s) (e\<^sub>1 # h)"
+| ret_tyapp_let [simp]: "StackState Return (Let e\<^sub>1 e\<^sub>2) (STyApp t # s) h \<leadsto>\<^sub>s 
+    StackState Eval e\<^sub>2 (STyApp t # SBind # s) (e\<^sub>1 # h)" 
+
+primrec is_final :: "stack_state \<Rightarrow> bool" where
+  "is_final (StackState m e s h) = (m = Return \<and> s = [])"
+
+theorem progress: "\<Sigma> hastype t \<Longrightarrow> is_final \<Sigma> \<or> (\<exists>\<Sigma>'. \<Sigma> \<leadsto>\<^sub>s \<Sigma>')"
+  proof (induction \<Sigma> t rule: typecheck_stack_state.induct)
+  case (tc_stack_state \<Gamma> s t t' e h m)
+    thus ?case
+      proof (induction m)
+      case Eval
+        thus ?case
+          proof (induction e)
+          case Var
+            thus ?case by simp
+          next case Abs
+            thus ?case by (metis ev_abs)
+          next case App
+            thus ?case by (metis ev_app)
+          next case Let
+            thus ?case by (metis ev_let)
+          next case Rec
+            thus ?case by (metis ev_app)
+          next case Proj
+            thus ?case by (metis ev_proj)
+          next case Inj 
+            thus ?case by (metis ev_inj)
+          next case Case
+            thus ?case by (metis ev_case)
+          next case Fold 
+            thus ?case by (metis ev_fold)
+          next case Unfold
+            thus ?case by (metis ev_unfold)
+          next case TyAbs
+            thus ?case by (metis ev_tyabs)
+          next case TyApp
+            thus ?case by (metis ev_tyapp)
+          next case TyLet
+            thus ?case by (metis ev_tylet)
+          qed
+      next case Return
+        thus ?case
+          proof (induction \<Gamma> s t t' rule: typecheck_stack.induct)
+          case (tcs_cons \<Gamma> f \<Gamma>' t t' s t'')
+            from tcs_cons have "\<Gamma> \<turnstile>\<^sub>s f : \<Gamma>',t \<rightarrow> t'" by simp
+            from tcs_cons have "\<Gamma> \<turnstile>\<^sub>s\<^sub>s s : t' \<rightarrow> t''" by simp
+            from tcs_cons have "[] ,\<Gamma> \<turnstile> e : t' \<Longrightarrow> h \<turnstile>\<^sub>h \<Gamma> \<Longrightarrow> s = [] \<or> (\<exists>a. StackState Return e s h \<leadsto>\<^sub>s a)" by simp
+            from tcs_cons have "[] ,\<Gamma>' \<turnstile> e : t" by simp
+            from tcs_cons have "h \<turnstile>\<^sub>h \<Gamma>'" by simp
+            from tcs_cons have "is_value e" by simp
+        
+        
+            have "StackState Return e (f # s) h \<leadsto>\<^sub>s \<Sigma>'" by simp
+            thus ?case by fastforce
+          qed simp_all
+      qed
+  qed
+
+theorem preservation: "\<Sigma> \<leadsto>\<^sub>s \<Sigma>' \<Longrightarrow> \<Sigma> hastype t \<Longrightarrow> \<Sigma>' hastype t"
+  proof (induction \<Sigma> \<Sigma>' rule: evaluate.induct)
+  case (ev_app e\<^sub>1 e\<^sub>2 s h)
+    then obtain \<Gamma> t\<^sub>1 t\<^sub>2 where "(\<Gamma> \<turnstile>\<^sub>s\<^sub>s s : t\<^sub>2 \<rightarrow> t) \<and> ([],\<Gamma> \<turnstile> e\<^sub>1 : Arrow t\<^sub>1 t\<^sub>2) \<and> 
+      ([],\<Gamma> \<turnstile> e\<^sub>2 : t\<^sub>1) \<and> (h \<turnstile>\<^sub>h \<Gamma>)" by fastforce
+    moreover hence "\<Gamma> \<turnstile>\<^sub>s\<^sub>s SApp e\<^sub>2 # s : Arrow t\<^sub>1 t\<^sub>2 \<rightarrow> t" by (metis tc_sapp tcs_cons)
+    ultimately show ?case by simp
+  qed simp_all
+
+end
