02Stack/TypecheckStack.thy
@@ -1,0 +1,87 @@
+theory TypecheckStack
+imports Stack "../01Expression/Typecheck"
+begin
+
+inductive typecheck_frame :: "type list \<Rightarrow> frame \<Rightarrow> type list \<Rightarrow> type \<Rightarrow> type \<Rightarrow> bool" 
+    (infix "\<turnstile>\<^sub>s _ : _,_ \<rightarrow>" 60) where
+  tc_sref [simp]: "lookup x \<Gamma> = Some t \<Longrightarrow> \<Gamma> \<turnstile>\<^sub>s SRef x : \<Gamma>,t \<rightarrow> t"
+| tc_sapp [simp]: "[],\<Gamma> \<turnstile> e : t' \<Longrightarrow> \<Gamma> \<turnstile>\<^sub>s SApp e : \<Gamma>,Arrow t' t \<rightarrow> t"
+| tc_sbind [simp]: "\<Gamma> \<turnstile>\<^sub>s SBind : t' # \<Gamma>,t \<rightarrow> t"
+| tc_sproj [simp]: "lookup l ts = Some t \<Longrightarrow> \<Gamma> \<turnstile>\<^sub>s SProj l : \<Gamma>,Record ts \<rightarrow> t"
+| tc_scase [simp]: "[],\<Gamma> \<turnstile>\<^sub>c cs : ts \<rightarrow> t \<Longrightarrow> \<Gamma> \<turnstile>\<^sub>s SCase t cs : \<Gamma>,Variant ts \<rightarrow> t"
+| tc_sunfold [simp]: "[k] \<turnstile>\<^sub>k t : Star \<Longrightarrow> 
+    \<Gamma> \<turnstile>\<^sub>s SUnfold t : \<Gamma>,Inductive k t \<rightarrow> subst\<^sub>t\<^sub>t 0 (Inductive k t) t"
+| tc_styapp [simp]: "[] \<turnstile>\<^sub>k t' : k \<Longrightarrow> \<Gamma> \<turnstile>\<^sub>s STyApp t' : \<Gamma>,Forall k t \<rightarrow> subst\<^sub>t\<^sub>t 0 t' t"
+
+inductive_cases [elim]: "\<Gamma> \<turnstile>\<^sub>s SRef x : \<Gamma>',t \<rightarrow> t'"
+inductive_cases [elim]: "\<Gamma> \<turnstile>\<^sub>s SApp e : \<Gamma>',t \<rightarrow> t'"
+inductive_cases [elim]: "\<Gamma> \<turnstile>\<^sub>s SBind : \<Gamma>',t \<rightarrow> t'"
+inductive_cases [elim]: "\<Gamma> \<turnstile>\<^sub>s SProj l : \<Gamma>',t \<rightarrow> t'"
+inductive_cases [elim]: "\<Gamma> \<turnstile>\<^sub>s SCase tt cs : \<Gamma>',t \<rightarrow> t'"
+inductive_cases [elim]: "\<Gamma> \<turnstile>\<^sub>s SUnfold tt : \<Gamma>',t \<rightarrow> t'"
+inductive_cases [elim]: "\<Gamma> \<turnstile>\<^sub>s STyApp tt : \<Gamma>',t \<rightarrow> t'"
+
+inductive typecheck_stack :: "type list \<Rightarrow> frame list \<Rightarrow> type \<Rightarrow> type \<Rightarrow> bool" 
+    (infix "\<turnstile>\<^sub>s\<^sub>s _ : _ \<rightarrow>" 60) where
+  tcs_nil [simp]: "[] \<turnstile>\<^sub>s\<^sub>s [] : t \<rightarrow> t"
+| tcs_cons [simp]: "\<Gamma> \<turnstile>\<^sub>s f : \<Gamma>',t \<rightarrow> t' \<Longrightarrow> \<Gamma> \<turnstile>\<^sub>s\<^sub>s s : t' \<rightarrow> t'' \<Longrightarrow> \<Gamma>' \<turnstile>\<^sub>s\<^sub>s f # s : t \<rightarrow> t''"
+
+inductive_cases [elim]: "\<Gamma> \<turnstile>\<^sub>s\<^sub>s [] : t \<rightarrow> t'"
+inductive_cases [elim]: "\<Gamma> \<turnstile>\<^sub>s\<^sub>s f # s : t \<rightarrow> t'"
+
+inductive typecheck_heap :: "expr list \<Rightarrow> type list \<Rightarrow> bool" 
+    (infix "\<turnstile>\<^sub>h" 60) where
+  tch_nil [simp]: "[] \<turnstile>\<^sub>h []"
+| tch_cons [simp]: "[],\<Gamma> \<turnstile> e : t \<Longrightarrow> h \<turnstile>\<^sub>h \<Gamma> \<Longrightarrow> e # h \<turnstile>\<^sub>h t # \<Gamma>"
+
+inductive_cases [elim]: "[] \<turnstile>\<^sub>h \<Gamma>"
+inductive_cases [elim]: "e # h \<turnstile>\<^sub>h \<Gamma>"
+inductive_cases [elim]: "h \<turnstile>\<^sub>h []"
+inductive_cases [elim]: "h \<turnstile>\<^sub>h t # \<Gamma>"
+
+inductive typecheck_stack_state :: "stack_state \<Rightarrow> type \<Rightarrow> bool" (infix "hastype" 60) where
+  tc_stack_state [simp]: "\<Gamma> \<turnstile>\<^sub>s\<^sub>s s : t \<rightarrow> t' \<Longrightarrow> [],\<Gamma> \<turnstile> e : t \<Longrightarrow> h \<turnstile>\<^sub>h \<Gamma> \<Longrightarrow> 
+    (m = Return \<longrightarrow> is_value e) \<Longrightarrow> StackState m e s h hastype t'"
+
+inductive_cases [elim]: "StackState m e s h hastype t"
+
+lemma [simp]: "h \<turnstile>\<^sub>h \<Gamma> \<Longrightarrow> lookup x \<Gamma> = Some t \<Longrightarrow> [],\<Gamma> \<turnstile> e : t \<Longrightarrow> update_at x e h \<turnstile>\<^sub>h \<Gamma>"
+  proof (induction h \<Gamma> arbitrary: x rule: typecheck_heap.induct)
+  case (tch_cons \<Gamma> e' t' h)
+    thus ?case
+      proof (induction x)
+      case 0
+        thus ?case by simp
+      next case (Suc x)
+        from Suc have "[] ,\<Gamma> \<turnstile> e' : t'" by simp
+        from Suc have "h \<turnstile>\<^sub>h \<Gamma>" by simp
+        from Suc have "[] ,\<Gamma> \<turnstile> e : t \<Longrightarrow> update_at x e h \<turnstile>\<^sub>h \<Gamma>" by simp
+        from Suc have "lookup x \<Gamma> = Some t" by simp
+        from Suc have "[] ,t' # \<Gamma> \<turnstile> e : t" by simp
+
+
+        have "[],\<Gamma> \<turnstile> e' : t' \<Longrightarrow> update_at x e h \<turnstile>\<^sub>h \<Gamma> \<Longrightarrow> 
+              e' # update_at x e h \<turnstile>\<^sub>h t' # \<Gamma>" by simp
+
+        have "e' # update_at x e h \<turnstile>\<^sub>h t' # \<Gamma>" by simp
+        thus ?case by simp
+      qed
+  qed simp_all
+
+lemma [simp]: "\<Gamma> \<turnstile>\<^sub>s\<^sub>s s : t \<rightarrow> t' \<Longrightarrow> [],\<Gamma> \<turnstile> e : t \<Longrightarrow> h \<turnstile>\<^sub>h \<Gamma> \<Longrightarrow> [],[] \<turnstile> unstack e s h : t'"
+  proof (induction \<Gamma> s t t' arbitrary: e h rule: typecheck_stack.induct)
+  case (tcs_cons \<Gamma> f \<Gamma>' t t' s t'')
+    thus ?case
+      proof (induction \<Gamma> f \<Gamma>' t t' rule: typecheck_frame.induct)
+      case (tc_sbind \<Gamma> t' t) 
+        moreover then obtain v h' where "h = v # h' \<and> ([],\<Gamma> \<turnstile> v : t') \<and> (h' \<turnstile>\<^sub>h \<Gamma>)" 
+          by fastforce
+        moreover from tc_sbind have "[],insert_at 0 t' \<Gamma> \<turnstile> e : t" by (induction \<Gamma>) simp_all
+        ultimately show ?case by auto
+      qed simp_all
+  qed simp_all
+
+lemma [simp]: "\<Sigma> hastype t \<Longrightarrow> [],[] \<turnstile> unstack_state \<Sigma> : t"
+  by (induction \<Sigma> t rule: typecheck_stack_state.induct) simp_all
+
+end
